p256: use four fixed-window method for point_mul_g

code/ecdsap256/Hacl.Impl.P256.PointMul.fst
@@ -15,20 +15,20 @@ open Hacl.Impl.P256.PointAdd
 open Hacl.Impl.P256.PointDouble
 
 //module LSeq = Lib.Sequence
-//module LE = Lib.Exponentiation
+module LE = Lib.Exponentiation
 module SE = Spec.Exponentiation
 module BE = Hacl.Impl.Exponentiation
-//module ME = Hacl.Impl.MultiExponentiation
+module ME = Hacl.Impl.MultiExponentiation
 //module PT = Hacl.Impl.PrecompTable
-//module SPT256 = Hacl.Spec.PrecompBaseTable256
-//module BD = Hacl.Spec.Bignum.Definitions
+module SPT256 = Hacl.Spec.PrecompBaseTable256
+module BD = Hacl.Spec.Bignum.Definitions
 
 module S = Spec.P256
 module SL = Spec.P256.Lemmas
 //module SM = Hacl.Spec.P256.Montgomery
 
 include Hacl.Impl.P256.Group
-//include Hacl.P256.PrecompTable
+include Hacl.P256.PrecompTable
 
 #set-options "--z3rlimit 50 --fuel 0 --ifuel 0"
 
@@ -62,12 +62,125 @@ let point_mul res scalar p =
   BE.lexp_fw_consttime 12ul 0ul mk_p256_concrete_ops 4ul (null uint64) p 4ul 256ul scalar res
 
 
+val precomp_get_consttime: BE.pow_a_to_small_b_st U64 12ul 0ul mk_p256_concrete_ops 4ul 16ul
+    (BE.table_inv_precomp 12ul 0ul mk_p256_concrete_ops 4ul 16ul)
+[@CInline]
+let precomp_get_consttime ctx a table bits_l tmp =
+  [@inline_let] let len = 12ul in
+  [@inline_let] let ctx_len = 0ul in
+  [@inline_let] let k = mk_p256_concrete_ops in
+  [@inline_let] let l = 4ul in
+  [@inline_let] let table_len = 16ul in
+
+  BE.lprecomp_get_consttime len ctx_len k l table_len ctx a table bits_l tmp
+
+
+inline_for_extraction noextract
+val point_mul_g_noalloc: out:point -> scalar:felem
+  -> q1:point -> q2:point
+  -> q3:point -> q4:point ->
+  Stack unit
+  (requires fun h ->
+    live h scalar /\ live h out /\ live h q1 /\
+    live h q2 /\ live h q3 /\ live h q4 /\
+    disjoint out scalar /\ disjoint out q1 /\ disjoint out q2 /\
+    disjoint out q3 /\ disjoint out q4 /\
+    disjoint q1 q2 /\ disjoint q1 q3 /\ disjoint q1 q4 /\
+    disjoint q2 q3 /\ disjoint q2 q4 /\ disjoint q3 q4 /\
+    as_nat h scalar < S.order /\
+    point_inv h q1 /\ refl (as_seq h q1) == g_aff /\
+    point_inv h q2 /\ refl (as_seq h q2) == g_pow2_64 /\
+    point_inv h q3 /\ refl (as_seq h q3) == g_pow2_128 /\
+    point_inv h q4 /\ refl (as_seq h q4) == g_pow2_192)
+  (ensures  fun h0 _ h1 -> modifies (loc out) h0 h1 /\
+    point_inv h1 out /\
+   (let (b0, b1, b2, b3) = SPT256.decompose_nat256_as_four_u64 (as_nat h0 scalar) in
+    S.to_aff_point (from_mont_point (as_point_nat h1 out)) ==
+    LE.exp_four_fw S.mk_p256_comm_monoid g_aff 64 b0 g_pow2_64 b1 g_pow2_128 b2 g_pow2_192 b3 4))
+
+let point_mul_g_noalloc out scalar q1 q2 q3 q4 =
+  [@inline_let] let len = 12ul in
+  [@inline_let] let ctx_len = 0ul in
+  [@inline_let] let k = mk_p256_concrete_ops in
+  [@inline_let] let l = 4ul in
+  [@inline_let] let table_len = 16ul in
+  [@inline_let] let bLen = 1ul in
+  [@inline_let] let bBits = 64ul in
+
+  let h0 = ST.get () in
+  recall_contents precomp_basepoint_table_w4 precomp_basepoint_table_lseq_w4;
+  let h1 = ST.get () in
+  precomp_basepoint_table_lemma_w4 ();
+  assert (table_inv_w4 (as_seq h1 q1) (as_seq h1 precomp_basepoint_table_w4));
+
+  recall_contents precomp_g_pow2_64_table_w4 precomp_g_pow2_64_table_lseq_w4;
+  let h1 = ST.get () in
+  precomp_g_pow2_64_table_lemma_w4 ();
+  assert (table_inv_w4 (as_seq h1 q2) (as_seq h1 precomp_g_pow2_64_table_w4));
+
+  recall_contents precomp_g_pow2_128_table_w4 precomp_g_pow2_128_table_lseq_w4;
+  let h1 = ST.get () in
+  precomp_g_pow2_128_table_lemma_w4 ();
+  assert (table_inv_w4 (as_seq h1 q3) (as_seq h1 precomp_g_pow2_128_table_w4));
+
+  recall_contents precomp_g_pow2_192_table_w4 precomp_g_pow2_192_table_lseq_w4;
+  let h1 = ST.get () in
+  precomp_g_pow2_192_table_lemma_w4 ();
+  assert (table_inv_w4 (as_seq h1 q4) (as_seq h1 precomp_g_pow2_192_table_w4));
+
+  let r1 = sub scalar 0ul 1ul in
+  let r2 = sub scalar 1ul 1ul in
+  let r3 = sub scalar 2ul 1ul in
+  let r4 = sub scalar 3ul 1ul in
+  Hacl.Spec.P256.Bignum.bn_v_is_as_nat (as_seq h0 scalar);
+  SPT256.lemma_decompose_nat256_as_four_u64_lbignum (as_seq h0 scalar);
+
+  ME.mk_lexp_four_fw_tables len ctx_len k l table_len
+    table_inv_w4 table_inv_w4 table_inv_w4 table_inv_w4
+    precomp_get_consttime
+    precomp_get_consttime
+    precomp_get_consttime
+    precomp_get_consttime
+    (null uint64) q1 bLen bBits r1 q2 r2 q3 r3 q4 r4
+    (to_const precomp_basepoint_table_w4)
+    (to_const precomp_g_pow2_64_table_w4)
+    (to_const precomp_g_pow2_128_table_w4)
+    (to_const precomp_g_pow2_192_table_w4)
+    out
+
+
+val lemma_exp_four_fw_local: b:BD.lbignum U64 4{BD.bn_v b < S.order} ->
+  Lemma (let (b0, b1, b2, b3) = SPT256.decompose_nat256_as_four_u64 (BD.bn_v b) in
+    LE.exp_four_fw S.mk_p256_comm_monoid g_aff 64 b0 g_pow2_64 b1 g_pow2_128 b2 g_pow2_192 b3 4 ==
+    S.to_aff_point (S.point_mul_g (BD.bn_v b)))
+
+let lemma_exp_four_fw_local b =
+ let cm = S.mk_p256_comm_monoid in
+  let (b0, b1, b2, b3) = SPT256.decompose_nat256_as_four_u64 (BD.bn_v b) in
+  let res = LE.exp_four_fw cm g_aff 64 b0 g_pow2_64 b1 g_pow2_128 b2 g_pow2_192 b3 4 in
+  assert (res == SPT256.exp_as_exp_four_nat256_precomp cm g_aff (BD.bn_v b));
+  SPT256.lemma_point_mul_base_precomp4 cm g_aff (BD.bn_v b);
+  assert (res == LE.pow cm g_aff (BD.bn_v b));
+  SE.exp_fw_lemma S.mk_p256_concrete_ops S.base_point 256 (BD.bn_v b) 4;
+  LE.exp_fw_lemma cm g_aff 256 (BD.bn_v b) 4;
+  assert (S.to_aff_point (S.point_mul_g (BD.bn_v b)) == LE.pow cm g_aff (BD.bn_v b))
+
+
 [@CInline]
 let point_mul_g res scalar =
   push_frame ();
-  let g = create_point () in
-  make_base_point g;
-  point_mul res scalar g;
+  let h0 = ST.get () in
+  let q1 = create_point () in
+  make_base_point q1;
+  let q2 = mk_proj_g_pow2_64 () in
+  let q3 = mk_proj_g_pow2_128 () in
+  let q4 = mk_proj_g_pow2_192 () in
+  proj_g_pow2_64_lseq_lemma ();
+  proj_g_pow2_128_lseq_lemma ();
+  proj_g_pow2_192_lseq_lemma ();
+  point_mul_g_noalloc res scalar q1 q2 q3 q4;
+  Hacl.Spec.P256.Bignum.bn_v_is_as_nat (as_seq h0 scalar);
+  lemma_exp_four_fw_local (as_seq h0 scalar);
   pop_frame ()
 
 
