code/ecdsap256/Hacl.P256.PrecompTable.fst
@@ -1,0 +1,295 @@
+module Hacl.P256.PrecompTable
+
+open FStar.HyperStack
+open FStar.HyperStack.ST
+open FStar.Mul
+
+open Lib.IntTypes
+open Lib.Buffer
+
+module ST = FStar.HyperStack.ST
+module LSeq = Lib.Sequence
+
+module LE = Lib.Exponentiation
+module SE = Spec.Exponentiation
+module SPT = Hacl.Spec.PrecompBaseTable
+module SPT256 = Hacl.Spec.PrecompBaseTable256
+module SPTK = Hacl.Spec.P256.PrecompTable
+
+module S = Spec.P256
+module SL = Spec.P256.Lemmas
+
+open Hacl.Impl.P256.Point
+include Hacl.Impl.P256.Group
+
+#set-options "--z3rlimit 50 --fuel 0 --ifuel 0"
+
+let proj_point_to_list p =
+  SPTK.proj_point_to_list_lemma p;
+  SPTK.proj_point_to_list p
+
+let lemma_refl x =
+  SPTK.proj_point_to_list_lemma x
+
+//-----------------
+
+inline_for_extraction noextract
+let proj_g_pow2_64 : S.proj_point =
+  [@inline_let]
+  let rX : S.felem = 0x000931f4ae428a4ad81ee0aa89cf5247ce85d4dd696c61b4bb9d4761e57b7fbe in
+  [@inline_let]
+  let rY : S.felem = 0x7e88e5e6a142d5c2269f21a158e82ab2c79fcecb26e397b96fd5b9fbcd0a69a5 in
+  [@inline_let]
+  let rZ : S.felem = 0x02626dc2dd5e06cd19de5e6afb6c5dbdd3e41dc1472e7b8ef11eb0662e41c44b in
+  (rX, rY, rZ)
+
+val lemma_proj_g_pow2_64_eval : unit ->
+  Lemma (SE.exp_pow2 S.mk_p256_concrete_ops S.base_point 64 == proj_g_pow2_64)
+
+let lemma_proj_g_pow2_64_eval () =
+  SPT256.exp_pow2_rec_is_exp_pow2 S.mk_p256_concrete_ops S.base_point 64;
+  let qX, qY, qZ = normalize_term (SPT256.exp_pow2_rec S.mk_p256_concrete_ops S.base_point 64) in
+  normalize_term_spec (SPT256.exp_pow2_rec S.mk_p256_concrete_ops S.base_point 64);
+  let rX : S.felem = 0x000931f4ae428a4ad81ee0aa89cf5247ce85d4dd696c61b4bb9d4761e57b7fbe in
+  let rY : S.felem = 0x7e88e5e6a142d5c2269f21a158e82ab2c79fcecb26e397b96fd5b9fbcd0a69a5 in
+  let rZ : S.felem = 0x02626dc2dd5e06cd19de5e6afb6c5dbdd3e41dc1472e7b8ef11eb0662e41c44b in
+  assert_norm (qX == rX /\ qY == rY /\ qZ == rZ)
+
+
+inline_for_extraction noextract
+let proj_g_pow2_128 : S.proj_point =
+  [@inline_let]
+  let rX : S.felem = 0x04c3aaf6c6c00704e96eda89461d63fd2c97ee1e6786fc785e6afac7aa92f9b1 in
+  [@inline_let]
+  let rY : S.felem = 0x14f1edaeb8e9c8d4797d164a3946c7ff50a7c8cd59139a4dbce354e6e4df09c3 in
+  [@inline_let]
+  let rZ : S.felem = 0x80119ced9a5ce83c4e31f8de1a38f89d5f9ff9f637dca86d116a4217f83e55d2 in
+  (rX, rY, rZ)
+
+val lemma_proj_g_pow2_128_eval : unit ->
+  Lemma (SE.exp_pow2 S.mk_p256_concrete_ops proj_g_pow2_64 64 == proj_g_pow2_128)
+
+let lemma_proj_g_pow2_128_eval () =
+  SPT256.exp_pow2_rec_is_exp_pow2 S.mk_p256_concrete_ops proj_g_pow2_64 64;
+  let qX, qY, qZ = normalize_term (SPT256.exp_pow2_rec S.mk_p256_concrete_ops proj_g_pow2_64 64) in
+  normalize_term_spec (SPT256.exp_pow2_rec S.mk_p256_concrete_ops proj_g_pow2_64 64);
+  let rX : S.felem = 0x04c3aaf6c6c00704e96eda89461d63fd2c97ee1e6786fc785e6afac7aa92f9b1 in
+  let rY : S.felem = 0x14f1edaeb8e9c8d4797d164a3946c7ff50a7c8cd59139a4dbce354e6e4df09c3 in
+  let rZ : S.felem = 0x80119ced9a5ce83c4e31f8de1a38f89d5f9ff9f637dca86d116a4217f83e55d2 in
+  assert_norm (qX == rX /\ qY == rY /\ qZ == rZ)
+
+
+inline_for_extraction noextract
+let proj_g_pow2_192 : S.proj_point =
+  [@inline_let]
+  let rX : S.felem = 0xc762a9c8ae1b2f7434ff8da70fe105e0d4f188594989f193de0dbdbf5f60cb9a in
+  [@inline_let]
+  let rY : S.felem = 0x1eddaf51836859e1369f1ae8d9ab02e4123b6f151d9b796e297a38fa5613d9bc in
+  [@inline_let]
+  let rZ : S.felem = 0xcb433ab3f67815707e398dc7910cc4ec6ea115360060fc73c35b53dce02e2c72 in
+  (rX, rY, rZ)
+
+val lemma_proj_g_pow2_192_eval : unit ->
+  Lemma (SE.exp_pow2 S.mk_p256_concrete_ops proj_g_pow2_128 64 == proj_g_pow2_192)
+
+let lemma_proj_g_pow2_192_eval () =
+  SPT256.exp_pow2_rec_is_exp_pow2 S.mk_p256_concrete_ops proj_g_pow2_128 64;
+  let qX, qY, qZ = normalize_term (SPT256.exp_pow2_rec S.mk_p256_concrete_ops proj_g_pow2_128 64) in
+  normalize_term_spec (SPT256.exp_pow2_rec S.mk_p256_concrete_ops proj_g_pow2_128 64);
+  let rX : S.felem = 0xc762a9c8ae1b2f7434ff8da70fe105e0d4f188594989f193de0dbdbf5f60cb9a in
+  let rY : S.felem = 0x1eddaf51836859e1369f1ae8d9ab02e4123b6f151d9b796e297a38fa5613d9bc in
+  let rZ : S.felem = 0xcb433ab3f67815707e398dc7910cc4ec6ea115360060fc73c35b53dce02e2c72 in
+  assert_norm (qX == rX /\ qY == rY /\ qZ == rZ)
+
+
+// let proj_g_pow2_64 : S.proj_point =
+//   normalize_term (SPT256.exp_pow2_rec S.mk_p256_concrete_ops S.base_point 64)
+
+// let proj_g_pow2_128 : S.proj_point =
+//   normalize_term (SPT256.exp_pow2_rec S.mk_p256_concrete_ops proj_g_pow2_64 64)
+
+// let proj_g_pow2_192 : S.proj_point =
+//   normalize_term (SPT256.exp_pow2_rec S.mk_p256_concrete_ops proj_g_pow2_128 64)
+
+
+inline_for_extraction noextract
+let proj_g_pow2_64_list : SPTK.point_list =
+  normalize_term (SPTK.proj_point_to_list proj_g_pow2_64)
+
+inline_for_extraction noextract
+let proj_g_pow2_128_list : SPTK.point_list =
+  normalize_term (SPTK.proj_point_to_list proj_g_pow2_128)
+
+inline_for_extraction noextract
+let proj_g_pow2_192_list : SPTK.point_list =
+  normalize_term (SPTK.proj_point_to_list proj_g_pow2_192)
+
+
+let proj_g_pow2_64_lseq : LSeq.lseq uint64 12 =
+  normalize_term_spec (SPTK.proj_point_to_list proj_g_pow2_64);
+  Seq.seq_of_list proj_g_pow2_64_list
+
+let proj_g_pow2_128_lseq : LSeq.lseq uint64 12 =
+  normalize_term_spec (SPTK.proj_point_to_list proj_g_pow2_128);
+  Seq.seq_of_list proj_g_pow2_128_list
+
+let proj_g_pow2_192_lseq : LSeq.lseq uint64 12 =
+  normalize_term_spec (SPTK.proj_point_to_list proj_g_pow2_192);
+  Seq.seq_of_list proj_g_pow2_192_list
+
+
+val proj_g_pow2_64_lemma: unit ->
+  Lemma (S.to_aff_point proj_g_pow2_64 == pow_point (pow2 64) g_aff)
+
+let proj_g_pow2_64_lemma () =
+  lemma_proj_g_pow2_64_eval ();
+  SPT256.a_pow2_64_lemma S.mk_p256_concrete_ops S.base_point
+
+
+val proj_g_pow2_128_lemma: unit ->
+  Lemma (S.to_aff_point proj_g_pow2_128 == pow_point (pow2 128) g_aff)
+
+let proj_g_pow2_128_lemma () =
+  lemma_proj_g_pow2_128_eval ();
+  lemma_proj_g_pow2_64_eval ();
+  SPT256.a_pow2_128_lemma S.mk_p256_concrete_ops S.base_point
+
+
+val proj_g_pow2_192_lemma: unit ->
+  Lemma (S.to_aff_point proj_g_pow2_192 == pow_point (pow2 192) g_aff)
+
+let proj_g_pow2_192_lemma () =
+  lemma_proj_g_pow2_192_eval ();
+  lemma_proj_g_pow2_128_eval ();
+  lemma_proj_g_pow2_64_eval ();
+  SPT256.a_pow2_192_lemma S.mk_p256_concrete_ops S.base_point
+
+
+let proj_g_pow2_64_lseq_lemma () =
+  normalize_term_spec (SPTK.proj_point_to_list proj_g_pow2_64);
+  proj_g_pow2_64_lemma ();
+  SPTK.proj_point_to_list_lemma proj_g_pow2_64
+
+
+let proj_g_pow2_128_lseq_lemma () =
+  normalize_term_spec (SPTK.proj_point_to_list proj_g_pow2_128);
+  proj_g_pow2_128_lemma ();
+  SPTK.proj_point_to_list_lemma proj_g_pow2_128
+
+
+let proj_g_pow2_192_lseq_lemma () =
+  normalize_term_spec (SPTK.proj_point_to_list proj_g_pow2_192);
+  proj_g_pow2_192_lemma ();
+  SPTK.proj_point_to_list_lemma proj_g_pow2_192
+
+
+let mk_proj_g_pow2_64 () =
+  createL proj_g_pow2_64_list
+
+let mk_proj_g_pow2_128 () =
+  createL proj_g_pow2_128_list
+
+let mk_proj_g_pow2_192 () =
+  createL proj_g_pow2_192_list
+
+//----------------
+
+///  window size = 4; precomputed table = [[0]G, [1]G, ..., [15]G]
+
+inline_for_extraction noextract
+let precomp_basepoint_table_list_w4: x:list uint64{FStar.List.Tot.length x = 192} =
+  normalize_term (SPT.precomp_base_table_list mk_p256_precomp_base_table S.base_point 15)
+
+let precomp_basepoint_table_lseq_w4 : LSeq.lseq uint64 192 =
+  normalize_term_spec (SPT.precomp_base_table_list mk_p256_precomp_base_table S.base_point 15);
+  Seq.seq_of_list precomp_basepoint_table_list_w4
+
+let precomp_basepoint_table_lemma_w4 () =
+  normalize_term_spec (SPT.precomp_base_table_list mk_p256_precomp_base_table S.base_point 15);
+  SPT.precomp_base_table_lemma mk_p256_precomp_base_table S.base_point 16 precomp_basepoint_table_lseq_w4
+
+let precomp_basepoint_table_w4:
+  x:glbuffer uint64 192ul{witnessed x precomp_basepoint_table_lseq_w4 /\ recallable x} =
+  createL_global precomp_basepoint_table_list_w4
+
+
+///  window size = 4; precomputed table = [[0]([pow2 64]G), [1]([pow2 64]G), ..., [15]([pow2 64]G)]
+
+inline_for_extraction noextract
+let precomp_g_pow2_64_table_list_w4: x:list uint64{FStar.List.Tot.length x = 192} =
+  normalize_term (SPT.precomp_base_table_list mk_p256_precomp_base_table proj_g_pow2_64 15)
+
+let precomp_g_pow2_64_table_lseq_w4 : LSeq.lseq uint64 192 =
+  normalize_term_spec (SPT.precomp_base_table_list mk_p256_precomp_base_table proj_g_pow2_64 15);
+  Seq.seq_of_list precomp_g_pow2_64_table_list_w4
+
+let precomp_g_pow2_64_table_lemma_w4 () =
+  normalize_term_spec (SPT.precomp_base_table_list mk_p256_precomp_base_table proj_g_pow2_64 15);
+  SPT.precomp_base_table_lemma mk_p256_precomp_base_table
+    proj_g_pow2_64 16 precomp_g_pow2_64_table_lseq_w4;
+  proj_g_pow2_64_lemma ()
+
+let precomp_g_pow2_64_table_w4:
+  x:glbuffer uint64 192ul{witnessed x precomp_g_pow2_64_table_lseq_w4 /\ recallable x} =
+  createL_global precomp_g_pow2_64_table_list_w4
+
+
+///  window size = 4; precomputed table = [[0]([pow2 128]G), [1]([pow2 128]G),...,[15]([pow2 128]G)]
+
+inline_for_extraction noextract
+let precomp_g_pow2_128_table_list_w4: x:list uint64{FStar.List.Tot.length x = 192} =
+  normalize_term (SPT.precomp_base_table_list mk_p256_precomp_base_table proj_g_pow2_128 15)
+
+let precomp_g_pow2_128_table_lseq_w4 : LSeq.lseq uint64 192 =
+  normalize_term_spec (SPT.precomp_base_table_list mk_p256_precomp_base_table proj_g_pow2_128 15);
+  Seq.seq_of_list precomp_g_pow2_128_table_list_w4
+
+let precomp_g_pow2_128_table_lemma_w4 () =
+  normalize_term_spec (SPT.precomp_base_table_list mk_p256_precomp_base_table proj_g_pow2_128 15);
+  SPT.precomp_base_table_lemma mk_p256_precomp_base_table
+    proj_g_pow2_128 16 precomp_g_pow2_64_table_lseq_w4;
+  proj_g_pow2_128_lemma ()
+
+let precomp_g_pow2_128_table_w4:
+  x:glbuffer uint64 192ul{witnessed x precomp_g_pow2_128_table_lseq_w4 /\ recallable x} =
+  createL_global precomp_g_pow2_128_table_list_w4
+
+
+///  window size = 4; precomputed table = [[0]([pow2 192]G), [1]([pow2 192]G),...,[15]([pow2 192]G)]
+
+inline_for_extraction noextract
+let precomp_g_pow2_192_table_list_w4: x:list uint64{FStar.List.Tot.length x = 192} =
+  normalize_term (SPT.precomp_base_table_list mk_p256_precomp_base_table proj_g_pow2_192 15)
+
+let precomp_g_pow2_192_table_lseq_w4 : LSeq.lseq uint64 192 =
+  normalize_term_spec (SPT.precomp_base_table_list mk_p256_precomp_base_table proj_g_pow2_192 15);
+  Seq.seq_of_list precomp_g_pow2_192_table_list_w4
+
+let precomp_g_pow2_192_table_lemma_w4 () =
+  normalize_term_spec (SPT.precomp_base_table_list mk_p256_precomp_base_table proj_g_pow2_192 15);
+  SPT.precomp_base_table_lemma mk_p256_precomp_base_table
+    proj_g_pow2_192 16 precomp_g_pow2_64_table_lseq_w4;
+  proj_g_pow2_192_lemma ()
+
+let precomp_g_pow2_192_table_w4:
+  x:glbuffer uint64 192ul{witnessed x precomp_g_pow2_192_table_lseq_w4 /\ recallable x} =
+  createL_global precomp_g_pow2_192_table_list_w4
+
+
+///  window size = 5; precomputed table = [[0]G, [1]G, ..., [31]G]
+
+inline_for_extraction noextract
+let precomp_basepoint_table_list_w5: x:list uint64{FStar.List.Tot.length x = 384} =
+  normalize_term (SPT.precomp_base_table_list mk_p256_precomp_base_table S.base_point 31)
+
+let precomp_basepoint_table_lseq_w5 : LSeq.lseq uint64 384 =
+  normalize_term_spec (SPT.precomp_base_table_list mk_p256_precomp_base_table S.base_point 31);
+  Seq.seq_of_list precomp_basepoint_table_list_w5
+
+let precomp_basepoint_table_lemma_w5 () =
+  normalize_term_spec (SPT.precomp_base_table_list mk_p256_precomp_base_table S.base_point 31);
+  SPT.precomp_base_table_lemma mk_p256_precomp_base_table S.base_point 32 precomp_basepoint_table_lseq_w5
+
+let precomp_basepoint_table_w5:
+  x:glbuffer uint64 384ul{witnessed x precomp_basepoint_table_lseq_w5 /\ recallable x} =
+  createL_global precomp_basepoint_table_list_w5
